No more locally nameless

theories/Global.v
@@ -7,7 +7,6 @@ Import Prenex Implicits.
 Require Import MPST.Atom.
 Require Import MPST.AtomSets.
 Require Import MPST.Forall.
-Require Import MPST.LNVar.
 Require Import MPST.Actions.
 
 Section Syntax.
@@ -17,15 +16,11 @@ Section Syntax.
    *)
   Inductive g_ty :=
   | g_end
-  | g_var (v : rvar)
+  | g_var (v : nat)
   | g_rec (G : g_ty)
   | g_msg (p : role) (q : role) (Ks : seq (lbl * (mty * g_ty))).
 
   Open Scope mpst_scope.
-
-  Arguments bv [_] _.
-  Notation gfv a := (g_var (fv a)).
-  Notation gbv n := (g_var (bv n)).
 
   Fixpoint depth_gty (a : g_ty) :=
     match a with
@@ -146,31 +141,17 @@ Section Syntax.
   Fixpoint g_open (d : nat) (G2 : g_ty) (G1 : g_ty) :=
     match G1 with
     | g_end => G1
-    | g_var v => open g_var d G2 v
+    | g_var v => if v == d then G2 else G1
     | g_rec G => g_rec (g_open d.+1 G2 G)
     | g_msg p q Ks =>
       g_msg p q [seq (K.lbl, (K.mty, g_open d G2 K.cnt)) | K <- Ks]
     end.
   Notation "{ k '~>' v } G":= (g_open k v G) (at level 30, right associativity).
-  Notation "G '^' v":= (g_open 0 (gfv v) G) (at level 30, right associativity).
+  Notation "G '^' v":= (g_open 0 (g_var v) G) (at level 30, right associativity).
 
-  Fixpoint g_close (v : atom) (d : nat) (G1 : g_ty) :=
-    match G1 with
-    | g_end => G1
-    | g_var gv => g_var (close v d gv)
-    | g_rec G => g_rec (g_close v d.+1 G)
-    | g_msg p q Ks => g_msg p q [seq (K.lbl, (K.mty, g_close v d K.cnt)) | K <- Ks]
-    end.
-  Notation "{ k '<~' v } G":= (g_close v k G) (at level 30, right associativity).
+  Definition unroll G := g_open 0 (g_rec G) G.
 
   Open Scope fset_scope.
-  Fixpoint g_fvar (G : g_ty) : {fset atom} :=
-    match G with
-    | g_var v => fvar v
-    | g_rec G => g_fvar G
-    | g_msg p q Ks => fsetUs [seq g_fvar K.cnt | K <- Ks]
-    | g_end => fset0
-    end.
 
   Lemma in_fold_has (A : choiceType) (x : A) (l : seq {fset A}) :
     (x \in fsetUs l) = has (fun s => x \in s) l.
@@ -186,74 +167,31 @@ Section Syntax.
     (x \notin fsetUs l) = all (fun s => x \notin s) l.
   Proof. by rewrite in_fold_has -all_predC. Qed.
 
-  Fixpoint g_fbvar (d : nat) (G : g_ty) : {fset nat} :=
+  Fixpoint g_fidx (d : nat) (G : g_ty) : {fset nat} :=
     match G with
-    | g_var v => fbvar d v
-    | g_rec G => g_fbvar d.+1 G
-    | g_msg p q Ks => fsetUs [seq g_fbvar d K.cnt | K <- Ks]
+    | g_var v => if v >= d then [fset v - d] else fset0
+    | g_rec G => g_fidx d.+1 G
+    | g_msg p q Ks => fsetUs [seq g_fidx d K.cnt | K <- Ks]
     | g_end => fset0
     end.
 
-  Definition g_lc (G : g_ty) := g_fbvar 0 G = fset0.
+  Definition g_lc (G : g_ty) := g_fidx 0 G = fset0.
 
-  Definition g_closed (G : g_ty) :=
-    (g_fbvar 0 G == fset0) && (g_fvar G == fset0).
+  Definition g_closed (G : g_ty) := g_fidx 0 G == fset0.
 
-  Lemma in_gfvar_gfv (a a' : atom) : (a \in g_fvar (gfv a')) = (a == a').
-  Proof.
-    rewrite /g_fvar; case: fset1P=>[->|].
-    - by rewrite eq_refl.
-    - by move=> /eqP/negPf->.
-  Qed.
-
-  Lemma gopen_gfv n X (a : atom) : g_open n X (gfv a) = gfv a.
-  Proof. by []. Qed.
-
-  Lemma gclose_gfv n X (a : atom) :
-    g_close X n (gfv a) = if X == a then (gbv n) else (gfv a).
-  Proof. by rewrite /g_close/close (fun_if g_var). Qed.
-
-  Lemma g_open_close X (G : g_ty) n : X \notin g_fvar G -> {n <~ X}{n ~> gfv X}G = G.
-  Proof.
-    elim/gty_ind1: G n =>//.
-    - by move=> v d /= H; rewrite open_fun /= (open_close d H).
-    - move=> G Ih d; rewrite /g_fvar -/(g_fvar _)=>/Ih-{Ih}Ih.
-      by rewrite -[in RHS](Ih d.+1).
-    - move=> p q Ks Ih n /= H; rewrite -map_comp/comp/=; congr g_msg.
-      elim: Ks H Ih => {p} {q} [//|/=[l [t G]] Ks Ih].
-      rewrite fsetUs_cons negb_or /= =>/andP-[X_G X_KS] IhKs.
-      rewrite (IhKs (l, (t, G)) (or_introl (Logic.eq_refl _)) n X_G) Ih //.
-      by move=> K KKs r H; apply: IhKs =>//; right.
-  Qed.
-
-  Lemma g_close_open n X (G : g_ty) : n \notin g_fbvar 0 G -> {n ~> gfv X}{n <~ X}G = G.
-  Proof.
-    move: {1 3}n (add0n n)=>n0; elim/gty_ind2: G 0 n =>///=.
-    - by move=> v n n1 <- H; rewrite addnC open_fun close_open.
-    - move=> G Ih d n Eq n_in; congr g_rec; apply: (Ih d.+1)=>//.
-      by rewrite -Eq.
-    - move=> p q Ks /Fa_lift-Fa d n Eq; rewrite notin_fold_all !all_map /preim/=.
-      move: (Fa d)=>{Fa}/Fa_lift/(_ n)/Fa_lift/(_ Eq)-Fa.
-      move=>/forallbP/(Fa_conj Fa){Fa}.
-      rewrite /SimplPred/= =>/Fa_app/Fa_map_eq-Ih.
-      rewrite -map_comp /comp/=; congr g_msg => {Eq d n0 p q}.
-      by elim: Ks Ih=>[//|/=[l [t G]] Ks Ih [-> /Ih->]].
-  Qed.
+  Fixpoint g_free_index (d : nat) (G : g_ty) : seq nat
+    :=
+    match G with
+    | g_end => [::]
+    | g_var v => if v >= d then [:: v - d] else [::]
+    | g_rec G => g_free_index d.+1 G
+    | g_msg p q Ks => flatten [seq g_free_index d K.cnt | K <- Ks]
+    end.
   Close Scope fset_scope.
 
-  Lemma g_depth_open (G : g_ty) X : depth_gty G = depth_gty (G^X).
-  Proof.
-    move: 0; elim/gty_ind2: G=>/=//.
-    + by move=>v n; rewrite open_fun.
-    + by move=> G Ih n; rewrite (Ih n.+1).
-    + move=> _ _ Gs /Fa_lift-Ih n; move: (Ih n) => {Ih}/Fa_map_eq.
-      rewrite -map_comp /comp/=.
-      by elim: Gs=>[//|/=[l G] Gs Ih []<- /Ih-{Ih}[<-]].
-  Qed.
-
   Lemma gfbvar_next n G :
-    g_fbvar n G == fset0 ->
-    g_fbvar n.+1 G = fset0.
+    g_fidx n G == fset0 ->
+    g_fidx n.+1 G = fset0.
   Proof.
     elim/gty_ind1: G n=>[//|v|G Ih|p q Ks Ih] n/=.
     - case: v=>//= m H; case: ifP=>// n_m; move: H.
@@ -263,54 +201,11 @@ Section Syntax.
       by rewrite fsetUs_fset0 member_map=> K M; move: (Ih K M n (H K M))=>->.
   Qed.
 
-  Lemma gopen_closed G :
-    g_closed (g_rec G) ->
-    g_closed (g_open 0 (g_rec G) G).
-  Proof.
-    rewrite/g_closed/==>/andP-[G_fbv /eqP-G_fv]; apply/andP; split=>[{G_fv}|{G_fbv}].
-    + have: g_fbvar 0 (g_rec G) == fset0 by [].
-      move: (g_rec G) => G' G'0.
-      elim/gty_ind1: G 0 G'0 G_fbv=>[//|v|G Ih|p q Ks Ih] n G'0/=.
-      - case: v=>[//|/= m]; case: ifP; first by rewrite -cardfs_eq0 cardfs1//.
-        case: ifP=>[/eqP<-//|/=]; case: ifP=>//.
-        by rewrite ltn_neqAle (rwP negPf)=>->->.
-      - by apply: (Ih n.+1); rewrite gfbvar_next.
-      - rewrite -map_comp/comp/=; move=>/fsetUs_fset0/member_map-H.
-        by apply/fsetUs_fset0/member_map=>K M; apply: Ih=>//; apply: H.
-    + move: G_fv=>/eqP-G_fv; have: g_fvar (g_rec G) == fset0 by [].
-      move: (g_rec G) => G' G'_fv.
-      elim/gty_ind1: G 0 G_fv =>[//|v |G Ih | p q Ks Ih] n /=.
-      - by case v=>//; case =>[|m]//=; case: ifP.
-      - by apply: Ih.
-      - rewrite -map_comp/comp !fsetUs_fset0 !member_map=> H K M.
-        by apply: Ih => //; apply: H.
-  Qed.
-
-  (* Induction scheme that takes into account that g_rec must be opened *)
-  Lemma gty_ind3 :
-    forall (P : g_ty -> Type),
-      P g_end ->
-      (forall v, P (g_var v)) ->
-      (forall G, (forall X (s : {fset atom}), X \notin s -> P (G ^ X)) ->
-                 P (g_rec G)) ->
-      (forall p q Ks, (forall K, K \in Ks -> P K.cnt) -> P (g_msg p q Ks)) ->
-      forall g : g_ty, P g.
-  Proof.
-    move=> P P_end P_var P_rec P_msg G.
-    move: {-1}(depth_gty G) (leqnn (depth_gty G))=> n; move: n G; elim.
-    + by case.
-    + move=>n Ih; case=>///=.
-      - by move=> G dG; apply: P_rec => X S _; apply: Ih; rewrite -g_depth_open.
-      - move=>p q Ks dKs; apply: P_msg=>K /(map_f (fun X => depth_gty X.cnt))/=.
-        move=>/in_maximum_leq-dG; move: (leq_trans dG dKs)=>{dG} {dKs}.
-        by apply: Ih.
-  Qed.
-
   Fixpoint guarded d G :=
     match G with
     | g_end
     | g_var _ => true
-    | g_rec G => if G is g_var (bv v)
+    | g_rec G => if G is g_var v
                  then v > d
                  else guarded d.+1 G
     | g_msg _ _ Ks => all (fun K => guarded 0 K.cnt) Ks
@@ -323,9 +218,9 @@ Section Syntax.
       Guarded d (g_var v)
   | G_rec_var d v :
       v > d ->
-      Guarded d (g_rec (gbv v))
+      Guarded d (g_rec (g_var v))
   | G_rec d G :
-      (forall v, G != gbv v) ->
+      (forall v, G != g_var v) ->
       Guarded d.+1 G ->
       Guarded d (g_rec G)
   | G_msg d p q Ks :
@@ -342,7 +237,7 @@ Section Syntax.
 
   Lemma grec_not_guarded d G' :
     ~ Guarded d.+1 G' ->
-    (forall v : nat, G' != gbv v) ->
+    (forall v : nat, G' != g_var v) ->
     ~ Guarded d (g_rec G').
   Proof.
     move=> N_GG' Ne; move: {-1}d (eq_refl d) {-1}(g_rec G') (eq_refl (g_rec G')).
@@ -361,26 +256,26 @@ Section Syntax.
     by rewrite Ih; do ! rewrite !eqE/=; rewrite -!eqE !andbA.
   Qed.
 
+  Lemma gty_not_var A G (f : nat -> A) (k : A) :
+    (forall v : nat, G != g_var v) ->
+    match G with | g_var v => f v | _ => k end = k.
+  Proof. by case: G =>// v /(_ v)/eqP. Qed.
+
   Lemma guardedP d G : reflect (Guarded d G) (guarded d G).
   Proof.
     move: G d; fix Ih 1; case=> [|v|G|p q Ks] d/=; try do ! constructor.
-    - move: {-1} G (eq_refl G) => G' Eq.
-      case: G' Eq=>[|[a|n]|G'|p q Ks]; try do ! constructor.
-      * case: (boolP (d < n))=>[d_lt_n|d_ge_n]; do ! constructor =>//.
-        move: {-1}d (eq_refl d) {-1}(g_rec (gbv n)) (eq_refl (g_rec (gbv n))).
-        move=> d' d_d' G' Eq_G H; case: H d_d' Eq_G=>//.
-        + move=> d0 v d_lt_n /eqP-H; move: H d_lt_n=><-{d0} d_lt_n H.
-          by move: H d_lt_n d_ge_n; do 2 rewrite !eqE/=; move=>/eqP<-->.
-        + move=> {d'} d' G'' Neq _ _; rewrite !eqE/=.
-          by case: G'' Neq=>// [[//|v]] /(_ v); rewrite eq_refl.
-      * move=> GG'; have: (forall v, G != gbv v) by move: GG'=>/eqP->.
-        move: GG'=>/eqP<-; case: (Ih G d.+1)=>[GG'|N_GG']; do ! constructor=>//.
-        by apply/grec_not_guarded.
-      * move=> GG'; have: (forall v, G != gbv v) by move: GG'=>/eqP->.
-        move: GG'=>/eqP<-; case: (Ih G d.+1)=>[GG'|N_GG']; do ! constructor=>//.
-        by apply/grec_not_guarded.
-    - elim: Ks=>[|K Ks]/=; try do ! constructor=>//.
-      case: (Ih K.cnt 0)=>[GK [GG|N_GG]|N_GK]/=; try do ! constructor=>//.
+    - have [[v->]|]: (sig (fun v => G = g_var v) + (forall v, G != g_var v))%type
+        by case: G=>[|v||]; try (by right); by (left; exists v).
+      * case: (boolP (d < v))=>[d_lt_n|d_ge_n]; do ! constructor =>//.
+        move=> GG; case E:_/GG d_ge_n=>[||d' v' H|d' G' H|]//.
+        + by move: E H=>[<-] ->.
+        + by move: E H=>[<-] /(_ v)/eqP.
+      * move=> H; rewrite (gty_not_var _ _ H); case: Ih; do ! constructor=>//.
+        move=> GG; case E:_/GG n=>[||d' v' F|d' G' _ F|]//.
+        + by move: E H=>[->] /(_ v')/eqP.
+        + by move: E F=>[->] F /(_ F).
+    - elim: Ks=>[|K Ks]//=; try do ! constructor=>//.
+      case: (Ih K.cnt 0)=>[GK [GG|N_GG]|N_GK]/=; do ! constructor=>//.
       * case Eq: (g_msg p q Ks) / GG=>// [d' p' q' Ks' GKs].
         move: Eq=>/eqP; rewrite alt_eq =>/andP-[_ Eq].
         by move: Eq GKs=>/eqP<-.
@@ -400,35 +295,35 @@ Section Syntax.
     | _ => 0
     end.
 
-  Fixpoint unroll d G :=
+  Fixpoint n_unroll d G :=
     match d with
     | 0 => G
     | d.+1 =>
       match G with
-      | g_rec G' => unroll d (g_open 0 G G')
+      | g_rec G' => n_unroll d (unroll G')
       | _ => G
       end
     end.
 
   Lemma guarded_match d G :
     match G with
-    | gbv v => d < v
+    | g_var v => d < v
     | _ => guarded d.+1 G
     end ->
-    (exists v, (G == gbv v) && (d < v)) \/
-    (forall v, (G != gbv v)) /\ guarded d.+1 G.
+    (exists v, (G == g_var v) && (d < v)) \/
+    (forall v, (G != g_var v)) /\ guarded d.+1 G.
   Proof.
     case: G=>[|[]||]//=; try by right.
-    by move=> n Eq; left; exists n; rewrite eq_refl.
+    by move=> n d_n; left; exists n.+1; rewrite eq_refl.
   Qed.
 
   Lemma guarded_recdepth d G m :
-    (forall v : nat, G != gbv v) ->
+    (forall v : nat, G != g_var v) ->
     guarded d G ->
     m < d ->
     forall G', rec_depth G = rec_depth ({m ~> G'} G).
   Proof.
-    elim/gty_ind1: G=>[|[a|n]|G Ih|p q Ks Ih]//= in d m *.
+    elim/gty_ind1: G=>[|n|G Ih|p q Ks Ih]//= in d m *.
     - by move=>/(_ n)/eqP.
     - move=> _ /guarded_match-[[n /andP-[/eqP->]/=]|[]].
       + move=> dn md G'; move: dn md; case: ifP=>[/eqP-> d_lt_n n_le_d|//].
@@ -437,15 +332,10 @@ Section Syntax.
         by rewrite -Ih.
   Qed.
 
-  Lemma gty_not_var G (b1 : nat -> bool) (b2 : bool) :
-    (forall v : nat, G != gbv v) ->
-    match G with | gbv v => b1 v | _ => b2 end = b2.
-  Proof. by case: G =>[|[|n /(_ n)/eqP]||]. Qed.
-
   Lemma guarded_depth_gt dG dG' G :
     guarded dG' G -> g_closed G -> guarded dG G.
   Proof.
-    rewrite /g_closed=> H /andP-[H' _]; move: 0 (leq0n dG') H H'.
+    rewrite /g_closed=> H H'; move: 0 (leq0n dG') H H'.
     elim/gty_ind1: G =>[|[a|n]|G Ih|p q Ks Ih]// in dG dG' *.
     move=> n n_le_dG'.
     move=>/guarded_match-[[m /andP-[/eqP->]]|[]].
@@ -453,22 +343,37 @@ Section Syntax.
       + by rewrite -cardfs_eq0 cardfs1.
       + move=>/(rwP negPf); rewrite -leqNgt => m_leq_n dG'_le_m.
         by move: (leq_ltn_trans n_le_dG' dG'_le_m); rewrite ltnNge m_leq_n.
-    - by move=>/gty_not_var/=->; apply: Ih.
+    - by move=>/(gty_not_var _ _)/=->; apply: Ih.
   Qed.
+
+  Lemma gopen_closed G :
+     g_closed (g_rec G) ->
+     g_closed (g_open 0 (g_rec G) G).
+   Proof.
+     rewrite/g_closed/==>G_fbv; have: g_fidx 0 (g_rec G) == fset0 by [].
+     move: (g_rec G) => G' G'0.
+     elim/gty_ind1: G 0 G'0 G_fbv=>[//|v|G Ih|p q Ks Ih] n G'0/=.
+     - move=> H; case: ifP=>[//|/=]; case: ifP=>//; move: H.
+       case: ifP=>//; first by rewrite -cardfs_eq0 cardfs1//.
+       rewrite ltn_neqAle =>/(rwP negPf); rewrite negb_and negbK eq_sym.
+       by move=>/orP-[->//|/negPf->].
+     - by apply: (Ih n.+1); rewrite gfbvar_next.
+     - rewrite -map_comp/comp/=; move=>/fsetUs_fset0/member_map-H.
+       by apply/fsetUs_fset0/member_map=>K M; apply: Ih=>//; apply: H.
+   Qed.
 
   Lemma closed_not_var G :
     g_closed G ->
-    forall v, G != gbv v.
+    forall v, G != g_var v.
   Proof.
-    rewrite /g_closed andbC =>/andP-[_].
-    by case: G=>//; case=>//= n; rewrite -cardfs_eq0 cardfs1.
+    by rewrite /g_closed; case: G=>//= n; rewrite -cardfs_eq0 cardfs1.
   Qed.
 
   Lemma open_not_var d G G' :
     g_closed G ->
-    (forall v, G' != gbv v) ->
-    forall v, {d ~> G} G' != gbv v.
-  Proof. by case: G'=>//; case=>//n _ /(_ n)/eqP. Qed.
+    (forall v, G' != g_var v) ->
+    forall v, {d ~> G} G' != g_var v.
+  Proof. by case: G'=>// n _ /(_ n)/eqP. Qed.
 
   Lemma guarded_open d1 d2 G G' :
     guarded 0 G' ->
@@ -476,14 +381,14 @@ Section Syntax.
     guarded d1 G ->
     guarded d1 ({d2 ~> G'} G).
   Proof.
-    elim/gty_ind1: G=>[|[a|n]|G Ih|p q Ks Ih]//= in d1 d2 *.
+    elim/gty_ind1: G=>[|n|G Ih|p q Ks Ih]//= in d1 d2 *.
     - by case: ifP=>// _ /guarded_depth_gt-H /H-{H}H.
     - move=>GG' CG'.
       move=> /guarded_match-[[v /andP-[/eqP-EG]]/=|[]].
       + move: EG=>->/=; case: ifP=>[/eqP _ _|//].
         rewrite (gty_not_var _ _ (closed_not_var CG')).
         by apply/(guarded_depth_gt _ GG' CG').
-      + move=> H; move: (open_not_var d2.+1 CG' H)=>/gty_not_var->.
+      + move=> H; move: (open_not_var d2.+1 CG' H)=>/(gty_not_var _ _)->.
         by apply/Ih.
     - move=> GG' CG'; elim: Ks=>[|K Ks IhK]//= in Ih *.
       move=>/andP-[GK GKs].
@@ -499,24 +404,25 @@ Section Syntax.
     elim/gty_ind1: G=>[|[a|n]|G Ih|p q Ks Ih]//= in d d' *.
     move=> d'_lt_d /guarded_match-[[v /andP-[/eqP->]]|[]].
     - by move=>/(ltn_trans d'_lt_d).
-    - by move/gty_not_var=>->; apply: Ih.
+    - by move/(gty_not_var _ _)=>->; apply: Ih.
   Qed.
 
   Lemma unroll_guarded G :
     g_closed G ->
     guarded 0 G ->
-    forall G', unroll (rec_depth G) G != g_rec G'.
+    forall G', n_unroll (rec_depth G) G != g_rec G'.
   Proof.
     move: {-2}(rec_depth G) (eq_refl (rec_depth G)) => n.
     elim: n => [|n Ih]/= in G *; case: G=>// G n_rd CG GG; move: n_rd.
     rewrite eqE/=-eqE => n_rd.
-    have /guarded_match-[[x /andP-[/eqP->/=]]|]: (guarded 0 (g_rec G)) by [].
-    - by case: ifP=>[/eqP<-//|x_ne0 d_le_x G']{Ih}{n_rd}; case: n.
+    have: (guarded 0 (g_rec G)) by [].
+    move=> /guarded_match-[[x /andP-[/eqP-G_v x_ne0]]|].
+    - move: G_v n_rd=>-> /eqP->/= G'; rewrite /unroll/=.
+      by move: x_ne0; case: ifP=>[/eqP->|].
     - move=>[G_ne_bv GG']; move: n_rd.
       rewrite (guarded_recdepth G_ne_bv GG' (ltn0Sn 0) (g_rec G)) =>n_rd.
-      apply/Ih=>//.
-      + by apply/gopen_closed.
-      + by move: (guarded_open 0 GG CG GG')=>/guarded_gt-H; apply/H.
+      apply/Ih=>//; first by apply/gopen_closed.
+      by move: (guarded_open 0 GG CG GG')=>/guarded_gt-H; apply/H.
   Qed.
 
   Close Scope mpst_scope.
@@ -544,7 +450,7 @@ Section Semantics.
   Open Scope mpst_scope.
 
   Lemma GUnroll_ind n iG cG :
-    GUnroll iG cG <-> GUnroll (unroll n iG) cG.
+    GUnroll iG cG <-> GUnroll (n_unroll n iG) cG.
   Proof.
     split.
     - elim: n =>// n Ih in iG cG *; case=>/=; try by constructor.
